<?xml version="1.0"?>
<rdf:RDF xmlns="https://www.inf.ufrgs.br/bdi/ontologies/geospr/geospr-simple.owl#"
     xml:base="https://www.inf.ufrgs.br/bdi/ontologies/geospr/geospr-simple.owl"
     xmlns:dc="http://purl.org/dc/elements/1.1/"
     xmlns:obo="http://purl.obolibrary.org/obo/"
     xmlns:owl="http://www.w3.org/2002/07/owl#"
     xmlns:rdf="http://www.w3.org/1999/02/22-rdf-syntax-ns#"
     xmlns:xml="http://www.w3.org/XML/1998/namespace"
     xmlns:xsd="http://www.w3.org/2001/XMLSchema#"
     xmlns:rdfs="http://www.w3.org/2000/01/rdf-schema#"
     xmlns:skos="http://www.w3.org/2004/02/skos/core#"
     xmlns:terms="http://purl.org/dc/terms/">
    <owl:Ontology rdf:about="https://www.inf.ufrgs.br/bdi/ontologies/geospr/geospr-simple.owl">
        <owl:versionIRI rdf:resource="https://www.inf.ufrgs.br/bdi/ontologies/geospr/releases/2024-04-06/geospr-simple.owl"/>
        <dc:contributor>Alcides Lopes</dc:contributor>
        <dc:contributor>Fernando Cicconeto</dc:contributor>
        <dc:contributor>Joel Luis Carbonera</dc:contributor>
        <dc:contributor>Luan Fonseca Garcia</dc:contributor>
        <dc:contributor>Lucas Valadares Vieira</dc:contributor>
        <dc:contributor>Mara Abel</dc:contributor>
        <dc:contributor>Renata dos Santos Alvarenga</dc:contributor>
        <terms:description>GeoSpatial Relations Ontology is an ontology that supports software applications in the determination of the physically possible spatial distribution of reservoir geological bodies.

Originally proposed in:

Cicconeto, F., Vieira, L. V., Abel, M., dos Santos Alvarenga, R., &amp; Carbonera, J. L. (2020). A Spatial Relation Ontology for Deep-Water Depositional System Description in Geology. In ONTOBRAS (pp. 35-47).

 https://ceur-ws.org/Vol-2728/paper3.pdf.</terms:description>
        <terms:license>https://creativecommons.org/licenses/by-nc/4.0/</terms:license>
        <terms:title>GeoSpatial Relations Ontology</terms:title>
        <owl:versionInfo>2024-04-06</owl:versionInfo>
    </owl:Ontology>
    


    <!-- 
    ///////////////////////////////////////////////////////////////////////////////////////
    //
    // Annotation properties
    //
    ///////////////////////////////////////////////////////////////////////////////////////
     -->

    


    <!-- http://purl.obolibrary.org/obo/IAO_0000115 -->

    <owl:AnnotationProperty rdf:about="http://purl.obolibrary.org/obo/IAO_0000115"/>
    


    <!-- http://purl.org/dc/elements/1.1/contributor -->

    <owl:AnnotationProperty rdf:about="http://purl.org/dc/elements/1.1/contributor"/>
    


    <!-- http://purl.org/dc/elements/1.1/identifier -->

    <owl:AnnotationProperty rdf:about="http://purl.org/dc/elements/1.1/identifier"/>
    


    <!-- http://purl.org/dc/terms/description -->

    <owl:AnnotationProperty rdf:about="http://purl.org/dc/terms/description"/>
    


    <!-- http://purl.org/dc/terms/license -->

    <owl:AnnotationProperty rdf:about="http://purl.org/dc/terms/license"/>
    


    <!-- http://purl.org/dc/terms/title -->

    <owl:AnnotationProperty rdf:about="http://purl.org/dc/terms/title"/>
    


    <!-- http://www.w3.org/2004/02/skos/core#definition -->

    <owl:AnnotationProperty rdf:about="http://www.w3.org/2004/02/skos/core#definition"/>
    


    <!-- http://www.w3.org/2004/02/skos/core#scopeNote -->

    <owl:AnnotationProperty rdf:about="http://www.w3.org/2004/02/skos/core#scopeNote"/>
    


    <!-- 
    ///////////////////////////////////////////////////////////////////////////////////////
    //
    // Object Properties
    //
    ///////////////////////////////////////////////////////////////////////////////////////
     -->

    


    <!-- http://purl.obolibrary.org/obo/BFO_0000124 -->

    <owl:ObjectProperty rdf:about="http://purl.obolibrary.org/obo/BFO_0000124">
        <owl:inverseOf rdf:resource="http://purl.obolibrary.org/obo/BFO_0000171"/>
        <dc:identifier>236-BFO</dc:identifier>
        <rdfs:label xml:lang="en">location of</rdfs:label>
        <skos:definition xml:lang="en">b location of c =Def c located in b</skos:definition>
        <skos:scopeNote xml:lang="en">Users that require more sophisticated representations of time are encouraged to import a temporal extension of BFO-Core provided by the BFO development team. See documentation for guidance: &lt;Link&gt;</skos:scopeNote>
    </owl:ObjectProperty>
    


    <!-- http://purl.obolibrary.org/obo/BFO_0000171 -->

    <owl:ObjectProperty rdf:about="http://purl.obolibrary.org/obo/BFO_0000171">
        <dc:identifier>234-BFO</dc:identifier>
        <rdfs:label xml:lang="en">located in</rdfs:label>
        <skos:definition xml:lang="en">b located in c =Def b is an independent continuant &amp; c is an independent &amp; neither is a spatial region &amp; there is some time t such that the spatial region which b occupies at t is continuant part of the spatial region which c occupies at t</skos:definition>
        <skos:scopeNote xml:lang="en">Users that require more sophisticated representations of time are encouraged to import a temporal extension of BFO-Core provided by the BFO development team. See documentation for guidance: &lt;Link&gt;</skos:scopeNote>
    </owl:ObjectProperty>
    


    <!-- https://www.inf.ufrgs.br/bdi/ontologies/GEOSPR_0000001 -->

    <owl:ObjectProperty rdf:about="https://www.inf.ufrgs.br/bdi/ontologies/GEOSPR_0000001">
        <owl:inverseOf rdf:resource="https://www.inf.ufrgs.br/bdi/ontologies/GEOSPR_0000004"/>
        <obo:IAO_0000115 xml:lang="en">A spatial relation between two Independent Continuants (BFO), x and y, in which x has a location greater than the location of y in the vertical axis corresponding to the same frame of reference. It is the inverse relation of Below.</obo:IAO_0000115>
        <rdfs:label xml:lang="en">above</rdfs:label>
    </owl:ObjectProperty>
    


    <!-- https://www.inf.ufrgs.br/bdi/ontologies/GEOSPR_0000002 -->

    <owl:ObjectProperty rdf:about="https://www.inf.ufrgs.br/bdi/ontologies/GEOSPR_0000002">
        <rdf:type rdf:resource="http://www.w3.org/2002/07/owl#SymmetricProperty"/>
        <obo:IAO_0000115 xml:lang="en">A symmetric spatial relation between two Independent Continuants (BFO) in which both share a part of the spatial regions they occupy.</obo:IAO_0000115>
        <rdfs:label xml:lang="en">spatially partially overlaps</rdfs:label>
    </owl:ObjectProperty>
    


    <!-- https://www.inf.ufrgs.br/bdi/ontologies/GEOSPR_0000003 -->

    <owl:ObjectProperty rdf:about="https://www.inf.ufrgs.br/bdi/ontologies/GEOSPR_0000003">
        <owl:inverseOf rdf:resource="https://www.inf.ufrgs.br/bdi/ontologies/GEOSPR_0000009"/>
        <obo:IAO_0000115 xml:lang="en">A spatial relation between two Independent Continuants(BFO), x and y, in which x has a location to the east of the location of y in the horizontal axis corresponding to the same frame of reference. It is the inverse relation of Right Of.</obo:IAO_0000115>
        <rdfs:label xml:lang="en">left of</rdfs:label>
    </owl:ObjectProperty>
    


    <!-- https://www.inf.ufrgs.br/bdi/ontologies/GEOSPR_0000004 -->

    <owl:ObjectProperty rdf:about="https://www.inf.ufrgs.br/bdi/ontologies/GEOSPR_0000004">
        <obo:IAO_0000115 xml:lang="en">A spatial relation between two Independent Continuants (BFO), x and y, in which x has a location lower than the location of y in the vertical axis corresponding to the same frame of reference. It is the inverse relation of Above.</obo:IAO_0000115>
        <rdfs:label xml:lang="en">below</rdfs:label>
    </owl:ObjectProperty>
    


    <!-- https://www.inf.ufrgs.br/bdi/ontologies/GEOSPR_0000005 -->

    <owl:ObjectProperty rdf:about="https://www.inf.ufrgs.br/bdi/ontologies/GEOSPR_0000005">
        <rdf:type rdf:resource="http://www.w3.org/2002/07/owl#SymmetricProperty"/>
        <obo:IAO_0000115 xml:lang="en">A symmetric spatial relation between two Independent Continuants (BFO) in which both do not share the same spatial region, either wholly or partially.</obo:IAO_0000115>
        <rdfs:label xml:lang="en">spatially discrete from</rdfs:label>
    </owl:ObjectProperty>
    


    <!-- https://www.inf.ufrgs.br/bdi/ontologies/GEOSPR_0000006 -->

    <owl:ObjectProperty rdf:about="https://www.inf.ufrgs.br/bdi/ontologies/GEOSPR_0000006">
        <rdfs:subPropertyOf rdf:resource="https://www.inf.ufrgs.br/bdi/ontologies/GEOSPR_0000005"/>
        <rdf:type rdf:resource="http://www.w3.org/2002/07/owl#SymmetricProperty"/>
        <obo:IAO_0000115 xml:lang="en">A symmetric subrelation of Spatially Discrete From between two Independent Continuants (BFO) whose external boundaries are adjacent.</obo:IAO_0000115>
        <rdfs:label xml:lang="en">externally connected with</rdfs:label>
    </owl:ObjectProperty>
    


    <!-- https://www.inf.ufrgs.br/bdi/ontologies/GEOSPR_0000007 -->

    <owl:ObjectProperty rdf:about="https://www.inf.ufrgs.br/bdi/ontologies/GEOSPR_0000007">
        <rdfs:subPropertyOf rdf:resource="https://www.inf.ufrgs.br/bdi/ontologies/GEOSPR_0000005"/>
        <rdf:type rdf:resource="http://www.w3.org/2002/07/owl#SymmetricProperty"/>
        <obo:IAO_0000115 xml:lang="en">A symmetric subrelation of Spatially Discrete From between two Independent Continuants (BFO) whose external boundaries are not adjacent.</obo:IAO_0000115>
        <rdfs:label xml:lang="en">spatially disconnected from</rdfs:label>
    </owl:ObjectProperty>
    


    <!-- https://www.inf.ufrgs.br/bdi/ontologies/GEOSPR_0000008 -->

    <owl:ObjectProperty rdf:about="https://www.inf.ufrgs.br/bdi/ontologies/GEOSPR_0000008">
        <rdf:type rdf:resource="http://www.w3.org/2002/07/owl#SymmetricProperty"/>
        <obo:IAO_0000115 xml:lang="en">A symmetric spatial relation between two Independent Continuants (BFO) in which both occupy precisely the same spatial region.</obo:IAO_0000115>
        <rdfs:label xml:lang="en">spatially identical to</rdfs:label>
    </owl:ObjectProperty>
    


    <!-- https://www.inf.ufrgs.br/bdi/ontologies/GEOSPR_0000009 -->

    <owl:ObjectProperty rdf:about="https://www.inf.ufrgs.br/bdi/ontologies/GEOSPR_0000009">
        <obo:IAO_0000115 xml:lang="en">A spatial relation between two Independent Continuants (BFO), x and y, in which x has a location to the west of the location of y in the horizontal axis corresponding to the same frame of reference. It is the inverse relation of Left Of.</obo:IAO_0000115>
        <rdfs:label xml:lang="en">right of</rdfs:label>
    </owl:ObjectProperty>
    


    <!-- https://www.inf.ufrgs.br/bdi/ontologies/GEOSPR_0000010 -->

    <owl:ObjectProperty rdf:about="https://www.inf.ufrgs.br/bdi/ontologies/GEOSPR_0000010">
        <owl:inverseOf rdf:resource="https://www.inf.ufrgs.br/bdi/ontologies/GEOSPR_0000011"/>
        <obo:IAO_0000115 xml:lang="en">A spatial relation between two Independent Continuants (BFO), x and y, in which x has a location that makes it nearer than y in the longitudinal axis corresponding to the same frame of reference. It is the inverse relation of Behind.</obo:IAO_0000115>
        <rdfs:label xml:lang="en">in front of</rdfs:label>
    </owl:ObjectProperty>
    


    <!-- https://www.inf.ufrgs.br/bdi/ontologies/GEOSPR_0000011 -->

    <owl:ObjectProperty rdf:about="https://www.inf.ufrgs.br/bdi/ontologies/GEOSPR_0000011">
        <obo:IAO_0000115 xml:lang="en">A spatial relation between two Independent Continuants(BFO), x and y, in which y has a location that makes it nearer than x in the longitudinal axis corresponding to the same frame of reference. It is the inverse relation of In Front Of.</obo:IAO_0000115>
        <rdfs:label xml:lang="en">behind</rdfs:label>
    </owl:ObjectProperty>
    


    <!-- https://www.inf.ufrgs.br/bdi/ontologies/GEOSPR_0000012 -->

    <owl:ObjectProperty rdf:about="https://www.inf.ufrgs.br/bdi/ontologies/GEOSPR_0000012">
        <rdfs:subPropertyOf rdf:resource="http://purl.obolibrary.org/obo/BFO_0000124"/>
        <owl:inverseOf rdf:resource="https://www.inf.ufrgs.br/bdi/ontologies/GEOSPR_0000015"/>
        <rdf:type rdf:resource="http://www.w3.org/2002/07/owl#TransitiveProperty"/>
        <obo:IAO_0000115 xml:lang="en">A transitive subrelation of Location Of (BFO) between two Independent Continuants (BFO), x and y, in which the spatial region that y occupies is entirely inside the spatial region that x occupies. It is the inverse relation of Proper Spatial Part Of.</obo:IAO_0000115>
        <rdfs:label xml:lang="en">has proper spatial part</rdfs:label>
    </owl:ObjectProperty>
    


    <!-- https://www.inf.ufrgs.br/bdi/ontologies/GEOSPR_0000013 -->

    <owl:ObjectProperty rdf:about="https://www.inf.ufrgs.br/bdi/ontologies/GEOSPR_0000013">
        <rdfs:subPropertyOf rdf:resource="https://www.inf.ufrgs.br/bdi/ontologies/GEOSPR_0000012"/>
        <owl:inverseOf rdf:resource="https://www.inf.ufrgs.br/bdi/ontologies/GEOSPR_0000016"/>
        <obo:IAO_0000115 xml:lang="en">A subrelation of Has Proper Spatial Part between two Independent Continuants (BFO) whose external boundaries are not adjacent. It is the inverse relation of Non-tangential Proper Spatial Part Of.</obo:IAO_0000115>
        <rdfs:label xml:lang="en">has non-tangential proper spatial part</rdfs:label>
    </owl:ObjectProperty>
    


    <!-- https://www.inf.ufrgs.br/bdi/ontologies/GEOSPR_0000014 -->

    <owl:ObjectProperty rdf:about="https://www.inf.ufrgs.br/bdi/ontologies/GEOSPR_0000014">
        <rdfs:subPropertyOf rdf:resource="https://www.inf.ufrgs.br/bdi/ontologies/GEOSPR_0000012"/>
        <owl:inverseOf rdf:resource="https://www.inf.ufrgs.br/bdi/ontologies/GEOSPR_0000017"/>
        <obo:IAO_0000115 xml:lang="en">A subrelation of Has Proper Spatial Part between two Independent Continuants (BFO) whose external boundaries are adjacent. It is the inverse relation of Tangential Proper Spatial Part Of.</obo:IAO_0000115>
        <rdfs:label xml:lang="en">has tangential proper spatial part</rdfs:label>
    </owl:ObjectProperty>
    


    <!-- https://www.inf.ufrgs.br/bdi/ontologies/GEOSPR_0000015 -->

    <owl:ObjectProperty rdf:about="https://www.inf.ufrgs.br/bdi/ontologies/GEOSPR_0000015">
        <rdfs:subPropertyOf rdf:resource="http://purl.obolibrary.org/obo/BFO_0000171"/>
        <rdf:type rdf:resource="http://www.w3.org/2002/07/owl#TransitiveProperty"/>
        <obo:IAO_0000115 xml:lang="en">A transitive subrelation of Located In (BFO) between two Independent Continuants (BFO), x and y, in which the spatial region that x occupies is entirely inside the spatial region that y occupies. It is the inverse relation of Has Proper Spatial Part.</obo:IAO_0000115>
        <rdfs:label xml:lang="en">proper spatial part of</rdfs:label>
    </owl:ObjectProperty>
    


    <!-- https://www.inf.ufrgs.br/bdi/ontologies/GEOSPR_0000016 -->

    <owl:ObjectProperty rdf:about="https://www.inf.ufrgs.br/bdi/ontologies/GEOSPR_0000016">
        <rdfs:subPropertyOf rdf:resource="https://www.inf.ufrgs.br/bdi/ontologies/GEOSPR_0000015"/>
        <obo:IAO_0000115 xml:lang="en">A subrelation of Proper Spatial Part Of between two Independent Continuants (BFO) whose external boundaries are not adjacent. It is the inverse relation of Has Non-tangential Proper Spatial Part.</obo:IAO_0000115>
        <rdfs:label xml:lang="en">non-tangential proper spatial part of</rdfs:label>
    </owl:ObjectProperty>
    


    <!-- https://www.inf.ufrgs.br/bdi/ontologies/GEOSPR_0000017 -->

    <owl:ObjectProperty rdf:about="https://www.inf.ufrgs.br/bdi/ontologies/GEOSPR_0000017">
        <rdfs:subPropertyOf rdf:resource="https://www.inf.ufrgs.br/bdi/ontologies/GEOSPR_0000015"/>
        <obo:IAO_0000115 xml:lang="en">A subrelation of Proper Spatial Part Of between two Independent Continuants (BFO) whose external boundaries are adjacent. It is the inverse relation of Has Tangential Proper Spatial Part.</obo:IAO_0000115>
        <rdfs:label xml:lang="en">tangential proper spatial part of</rdfs:label>
    </owl:ObjectProperty>
</rdf:RDF>



<!-- Generated by the OWL API (version 4.5.26) https://github.com/owlcs/owlapi -->

